\documentclass[a4paper]{article} 
\usepackage[english]{babel} 
\usepackage[utf8x]{inputenc} 
\usepackage[T1]{fontenc} 
\usepackage{ragged2e} 
\usepackage{amsmath} 
\usepackage[a4paper,top=3cm,bottom=2cm,left=3cm,right=3cm,marginparwidth=1.75cm]{geometry} 
\begin{document} 
\section*{equation.tex} 
\allowdisplaybreaks 
\begin{flalign*} 
\dot{x}_1 &= x_{2}\\\dot{x}_2 &= c_{1}\cdot \cos(x_{1}) + c_{2}\cdot g_{1}(\vec{x})\cdot x_{3} - c_{2}\cdot g_{2}(\vec{x})\cdot x_{4}\\\ddot{x}_2 &= -c_{1}\cdot \sin(x_{1})\cdot \dot{x}_1(\vec{x}) + c_{2}\cdot dg_{1}(\vec{x})\cdot \dot{x}_1(\vec{x})\cdot x_{3} + c_{2}\cdot g_{1}(\vec{x})\cdot \dot{x}_3(\vec{x})\\&\hspace{1.5em} 					- c_{2}\cdot dg_{2}(\vec{x})\cdot \dot{x}_1(\vec{x})\cdot x_{4} - c_{2}\cdot g_{2}(\vec{x})\cdot \dot{x}_4(\vec{x})\\\dot{x}_3 &= g_{3}(\vec{x})\cdot g_{5}(\vec{x}) - c_{3}\cdot g_{3}(\vec{x})\cdot x_{7}\\\dot{x}_4 &= g_{4}(\vec{x})\cdot g_{6}(\vec{x}) - c_{4}\cdot g_{4}(\vec{x})\cdot x_{8}\\\dot{x}_5 &= x_{7}\\\dot{x}_6 &= x_{8}\\\dot{x}_7 &= c_{5}\cdot x_{3} - c_{6}\cdot g_{7}(\vec{x})\cdot u_{1} - c_{6}\cdot g_{8}(\vec{x}) - c_{7}\cdot x_{7} \\&\hspace{1.5em} 	c_{8}\cdot x_{7}^{2}/x_{5}\\\dot{x}_8 &= c_{9}\cdot x_{4} - c_{10}\cdot g_{10}(\vec{x})\cdot u_{2} - c_{10}\cdot g_{9}(\vec{x}) - c_{11}\cdot x_{8} \\&\hspace{1.5em} 	c_{12}\cdot x_{8}^{2}/x_{6}\\&\hspace{1.5em} \\&\hspace{1.5em} \\	g_{1} &= r_{1}(x_{1}) #\\	dg_{1} &= r'_{1}(x_{1})\\	d2g_{1} &= r''_{1}(x_{1})\\	g_{2} &= r_{2}(x_{1}) #\\	dg_{2} &= r'_{2}(x_{1})\\	d2g_{2} &= r''_{2}(x_{1})\\	g_{3} &= cT\cdot (1-\text{exp}(-x_{3}/(cT\cdot kT))) #\\	dg_{3} &= \text{exp}(-x_{3}/(cT\cdot kT))/kT\\	g_{4} &= cT\cdot (1-\text{exp}(-x_{4}/(cT\cdot kT))) #\\	dg_{4} &= \text{exp}(-x_{4}/(cT\cdot kT))/kT\\	g_{5} &= np.sign(-dg_{1}(\vec{x})\cdot x_{2})\cdot x_{2}\cdot np.sqrt(dg_{1}(\vec{x})^{2} + g_{1}(\vec{x})^{2}) # Should be g_{4}\\	dg_{5} &=\\&\hspace{1.5em} 		np.sign(-dg_{1}(\vec{x})\cdot x_{2})\cdot (\dot{x}_2(\vec{x})\cdot np.sqrt(dg_{1}(\vec{x})^{2} + g_{1}(\vec{x})^{2}) +\\&\hspace{1.5em} 			(x_{2}^{2}\cdot dg_{1}(\vec{x})\cdot (d2g_{1}(\vec{x}) + g_{1}(\vec{x})))/np.sqrt(dg_{1}(\vec{x})^{2} + g_{1}(\vec{x})^{2}))\\	g_{6} &= np.sign(-dg_{2}(x_{1})\cdot x_{2})\cdot x_{2}\cdot np.sqrt(dg_{2}(x_{1})^{2} + g_{2}(x_{1})^{2}) # Should be g_{5}\\	dg_{6} &= \\&\hspace{1.5em} 		np.sign(-dg_{2}(\vec{x})\cdot x_{2})\cdot (\dot{x}_2(\vec{x})\cdot np.sqrt(dg_{2}(\vec{x})^{2}+ g_{2}(\vec{x})^{2}) +\\&\hspace{1.5em} 			(x_{2}^{2}\cdot dg_{2}(\vec{x})\cdot (d2g_{2}(\vec{x}) + g_{2}(\vec{x})))/np.sqrt(dg_{2}(\vec{x})^{2} + g_{2}(\vec{x})^{2}))\\	g_{7} &= \\&\hspace{1.5em} 		35\cdot PCSA1\\&\hspace{1.5em} 			\cdot \text{exp}(-abs(((x_{5}/lo1)\cdot \cdot β-1)/ω)\cdot \cdot ρ)\\				\cdot np.piecewise(x_{7},[x_{7}<&=0, x_{7}>0],\\&\hspace{1.5em} 					[lambda x_{7}: (V_max - x_{7}/lo1)/(V_max + (cv0 + cv1\cdot (x_{5}/lo1)\cdot (x_{7}/lo1))),\\&\hspace{1.5em} 					lambda x_{7}: (bv-(av0 + av1\cdot (x_{5}/lo1) + av2\cdot (x_{5}/lo1)^{2})\cdot (x_{7}/lo1))/(bv + (x_{7}/lo1))]) \\&\hspace{1.5em} 						# Should be g_{6}\\	g_{8} &= c_1\cdot k_1\cdot \text{ln}(\text{exp}(((x_{5}/lo1)-Lr1)/k_1) + 1) + η\cdot (x_{7}/lo1) # Should be g_{7}\\	g_{9} &= c_1\cdot k_1\cdot \text{ln}(\text{exp}(((x_{6}/lo2)-Lr1)/k_1) + 1) + η\cdot (x_{8}/lo2)\\	g_{10} &= \\&\hspace{1.5em} 		35\cdot PCSA2\\&\hspace{1.5em} 			\cdot \text{exp}(-abs(((x_{6}/lo2)\cdot \cdot β-1)/ω)\cdot \cdot ρ)\\				\cdot np.piecewise(x_{8},[x_{8}<&=0, x_{8}>0],\\&\hspace{1.5em} 					[lambda x_{8}: (V_max - x_{8}/lo2)/(V_max + (cv0 + cv1\cdot (x_{6}/lo2)\cdot (x_{8}/lo2))),\\&\hspace{1.5em} 					lambda x_{8}: (bv-(av0 + av1\cdot (x_{6}/lo2) + av2\cdot (x_{6}/lo2)^{2})\cdot (x_{8}/lo2))/(bv + (x_{8}/lo2))]) \\\end{flalign*} 
\end{document}